# For each of these sets of premises, express the statements in predicate logic and draw relevant conclusions, explaining the rules of inference used.

## a. 
### Premises:
1. ∀x (I(x) → L(x))  (All insects have six legs.)
2. I(d)  (Dragonflies are insects.)
3. ¬L(s)  (Spiders do not have six legs.)
4. E(s, d)  (Spiders eat dragonflies.)

### Conclusions:
- L(d)  (Dragonflies have six legs.)
- ¬I(s)  (Spiders are not insects.)

### Rules of Inference:
- **Universal Instantiation:** From premise 1, since dragonflies are insects (premise 2), we conclude L(d).
- **Contradiction:** From L(d) and premise 3, we conclude ¬I(s) since spiders do not have six legs.

## b.
### Premises:
1. ∀x (S(x) → I(x))  (Every student has an Internet account.)
2. ¬I(a)  (Akash does not have an Internet account.)
3. I(s)  (Sneha has an Internet account.)

### Conclusions:
- ¬S(a)  (Akash is not a student.)

### Rules of Inference:
- **Universal Instantiation:** From premise 1, we can infer S(a) → I(a).
- **Modus Tollens:** Since ¬I(a) (premise 2), we conclude ¬S(a).

## c.
### Premises:
1. ∀x (H(x) → ¬T(x))  (All foods that are healthy to eat do not taste good.)
2. H(t)  (Tofu is healthy to eat.)
3. ∀x (T(x) → E(x))  (You only eat what tastes good.)
4. ¬E(t)  (You do not eat tofu.)
5. ¬H(c)  (Cheeseburgers are not healthy to eat.)

### Conclusions:
- ¬E(c)  (You do not eat cheeseburgers.)

### Rules of Inference:
- **Universal Instantiation:** From premise 1, since H(t) (premise 2), it follows ¬T(t).
- **Contradiction:** From premise 3 and ¬T(t), we conclude ¬E(t).
- **Indirect Reasoning:** Since cheeseburgers are not healthy (premise 5), we cannot directly conclude ¬E(c), but we consider the context of healthy versus unhealthy foods.

## d.
### Premises:
1. D ∨ H  (I am either dreaming or hallucinating.)
2. ¬D  (I am not dreaming.)
3. H → E  (If I am hallucinating, I see elephants running down the road.)

### Conclusions:
- H  (I am hallucinating.)
- E  (I see elephants running down the road.)

### Rules of Inference:
- **Disjunctive Syllogism:** From D ∨ H and ¬D, we conclude H.
- **Modus Ponens:** Since H (from the previous conclusion), we apply premise 3 to conclude E.